fix precondition and reduce to two cheats

examples/riscv/common/bir_symbLib.sig
@@ -6,6 +6,7 @@ sig
   val mem_addrs_prog_disj_tm : string -> term;
 
   val mem_addrs_aligned_prog_disj_tm : string -> term;
+  val mem_addrs_aligned_prog_disj_riscv_tm : term -> term;
 
   val pre_vals_reg_tm : string -> string -> term;
 
